src/cbor/pulse/raw/CBOR.Pulse.API.Det.Type.fst
@@ -8,3 +8,4 @@ let cbor_det_array_iterator_t = CBOR.Pulse.Raw.Read.cbor_array_iterator
 let cbor_det_map_iterator_t = CBOR.Pulse.Raw.Read.cbor_map_iterator
 let cbor_det_array_append_cell_t = ML.cbor_raw_mixed_list Raw.cbor_raw
 let cbor_det_map_entry_insert_cell_t = ML.cbor_raw_mixed_list Raw.cbor_map_entry
+let cbor_det_array_t = Raw.cbor_mixed_list_array
